src/xor/tseitin.lean
@@ -1,0 +1,139 @@
+/-
+This file contains the development of the Tseitin encoding for XOR
+
+Authors: Cayden Codel, Jeremy Avidgad, Marijn Heule
+Carnegie Mellon University
+-/
+
+import cnf.literal
+import cnf.clause
+import cnf.cnf
+import xor.xor
+
+import data.list.basic
+import data.list.min_max
+
+open literal
+open clause
+open cnf
+open xor_gate
+
+open list
+
+namespace tseitin_xor
+
+lemma dropn_len {α : Type} {n : nat} {a : α} {l : list α} : n > 1 → length l > n → length (l.drop n ++ [a]) < length l :=
+begin
+  intros hn hl,
+  induction l with x xs ih,
+  { simp [lt_trans hn hl] at hl, contradiction },
+  { by_cases length xs = n,
+    { simp [h, gt.lt hn] },
+    { simp at hl,
+      have red := ih (gt.lt (array.push_back_idx hl (ne.symm h))), -- strange theorem
+      simp [nat.sub_add_eq_add_sub (nat.lt_succ_iff.mp hl)] at red,
+      simp [red] } }
+end
+
+-- We start with the instance of pooling number n = 3
+-- The n provided is the greatest element in l, so that new variables can be created
+-- The well_founded had to be used because of the growing n variable
+-- Unfold didn't work until I provided a nil case - intentional?
+def tseitin_xor3 : list literal → nat → cnf
+| [] _ := [[]]
+| l n := 
+    if h : length l ≤ 3 then xor_cnf l
+    else
+      have length (l.drop 3 ++ [Pos (n + 1)]) < length l, 
+        from (dropn_len (nat.succ 0).one_lt_succ_succ (not_le.mp h)),
+      xor_cnf (l.take 3 ++ [Neg (n + 1)]) ++ (tseitin_xor3 (l.drop 3 ++ [Pos (n + 1)]) (n + 1))
+using_well_founded {
+  rel_tac := λ a b, `[exact ⟨_, measure_wf (λ σ, list.length σ.fst)⟩],
+  dec_tac := tactic.assumption
+}
+
+lemma tseitin_xor3_base_case {ls : list literal} (n : nat) (h : length ls ≤ 3) :
+  tseitin_xor3 ls n = xor_cnf ls :=
+begin
+  rcases list_by_cases ls with (rfl | ⟨l, ls, rfl⟩),
+  { simp [tseitin_xor3, xor_cnf] },
+  { unfold tseitin_xor3, simp [h] }
+end
+
+-- Big theorem
+-- Modify to state that the greatest element of ls is its length
+-- TODO max var operates on clauses, but this is a list literal, clean up types later
+theorem tseitin_xor3_correct (α : assignment) : ∀ {ls : list literal}, ∀ {n : nat},
+  (map var ls).nodup → n = max_var ls → cnf.eval α (xor_cnf ls) = cnf.eval α (tseitin_xor3 ls n)
+| []   n := by { simp [xor_cnf, tseitin_xor3] }
+| [l]  n := begin
+  intros _ hmax,
+  have hlen : length [l] = 1, simp [length],
+  rw tseitin_xor3_base_case n (eq.trans_le hlen (nat.one_le_bit1 1))
+end
+| (l₁ :: [l₂]) n := begin
+  intros _ _,
+  have hlen : length (l₁ :: [l₂]) = 2, simp [length],
+  rw tseitin_xor3_base_case n (eq.trans_le hlen (nat.le_succ 2))
+end
+| (l₁ :: l₂ :: [l₃]) n := begin
+  intros _ _,
+  have hlen : length (l₁ :: l₂ :: [l₃]) = 3, simp [length],
+  rw tseitin_xor3_base_case n (eq.symm hlen).ge
+end
+| (l₁ :: l₂ :: l₃ :: l₄ :: l) n := begin
+  intros hnodup hmax,
+  have : 3 < 4, from nat.lt.base 3,
+  have : 3 < (length l) + 4, from nat.lt_add_left 3 4 (length l) this,
+  have hlen : (length l) + 1 + 1 + 1 + 1 > 3, simp [length, this],
+  have hlen2 : ¬((length l) + 1 + 1 + 1 + 1 ≤ 3), from not_le.mpr this,
+  unfold tseitin_xor3,
+  simp [hlen2],
+  have hnodup_original := hnodup,
+  rw map_cons at hnodup,
+  rw map_cons at hnodup,
+  rw map_cons at hnodup,
+  have t1 := nodup_of_nodup_cons hnodup,
+  have t2 := nodup_of_nodup_cons t1,
+  have t3 := nodup_of_nodup_cons t2,
+
+  have : (l₁ :: l₂ :: l₃ :: l₄ :: l) ≠ [], from cons_ne_nil l₁ (l₂ :: l₃ :: l₄ :: l),
+  have ngt : n + 1 > n, from lt_add_one n,
+
+  have s1 : max_var (l₂ :: l₃ :: l₄ :: l) ≤ max_var (l₁ :: l₂ :: l₃ :: l₄ :: l), 
+    from max_var_le_max_var_cons _ _,
+  have s2 : max_var (l₃ :: l₄ :: l) ≤ max_var (l₂ :: l₃ :: l₄ :: l),
+    from max_var_le_max_var_cons _ _,
+  have s3 : max_var (l₄ :: l) ≤ max_var (l₃ :: l₄ :: l),
+    from max_var_le_max_var_cons _ _,
+  have s23 : max_var (l₄ :: l) ≤ max_var (l₂ :: l₃ :: l₄ :: l),
+    from le_trans s3 s2,
+  have s13 : max_var (l₄ :: l) ≤ max_var (l₁ :: l₂ :: l₃ :: l₄ :: l),
+    from le_trans s23 s1,
+  rw ← hmax at s13,
+  have succn_gt : n + 1 > max_var (l₄ :: l), from gt_of_gt_of_ge ngt s13,
+  have : (Neg (n + 1)).var = n + 1, simp [var],
+
+  have smallnodup : (map var (l₁ :: l₂ :: l₃ :: [Neg (n + 1)])).nodup,
+  { sorry },
+  have newnodup : (map var (l₄ :: (l ++ [Pos (n + 1)]))).nodup,
+  { sorry },
+  have newmaxvar : n + 1 = max_var (l₄ :: (l ++ [Pos (n + 1)])),
+  { sorry },
+
+
+  have ihred := tseitin_xor3_correct newnodup newmaxvar,
+  rw cnf.eval_concat,
+  rw ← ihred,
+  rw xor_cnf_correct α hnodup_original,
+  rw xor_cnf_correct α newnodup,
+  rw xor_cnf_correct α smallnodup,
+  simp [xor_gate.eval_cons, xor_gate.eval_concat],
+  rcases bool_by_cases (eval α (Pos (n + 1))) with htt | hff,
+  {
+    simp [literal.eval] at htt,
+    simp [htt, bxor_ff, literal.eval],
+  }
+end
+
+end tseitin_xor
